Moved utility lemma out of resource file

fairis/map_included_utils.v
@@ -153,3 +153,333 @@ Proof.
   exists v2. split; [|done].
   by apply map_filter_lookup_Some_2.
 Qed.
+
+Lemma map_included_subseteq_r `{∀ A, Lookup K A (MAP A)} {A}
+      (R : relation A) (m1 m2 m3 : MAP A) :
+  m2 ⊆ m3 → map_included R m1 m2 → map_included R m1 m3.
+Proof.
+  rewrite /subseteq /map_subseteq !map_included_spec.
+  intros Hle1 Hle2.
+  intros k v1 HSome.
+  apply Hle2 in HSome as [v2 [HSome HR]].
+  apply Hle1 in HSome as [v3 [HSome HR']].
+  exists v3. split; [done|].
+  by subst.
+Qed.
+
+Definition map_agree_R `{∀ A, Lookup K A (MAP A)} {A B}
+           (R : A → B → Prop) (m1 : MAP A) (m2 : MAP B) :=
+  map_relation R (λ _, False) (λ _, False) m1 m2.
+
+Lemma map_agree_R_spec `{∀ A, Lookup K A (MAP A)} {A}
+      (R : relation A) (m1 m2 : MAP A) :
+  map_agree_R R m1 m2 ↔
+  (∀ k v1, m1 !! k = Some v1 → ∃ v2, m2 !! k = Some v2 ∧ R v1 v2) ∧
+  (∀ k v2, m2 !! k = Some v2 → ∃ v1, m1 !! k = Some v1 ∧ R v1 v2).
+Proof.
+  rewrite /map_agree_R /map_relation /option_relation. split.
+  - intros HR. split.
+    + intros k v HSome. specialize (HR k). rewrite HSome in HR.
+      destruct (m2 !! k); [by eauto|done].
+    + intros k v HSome. specialize (HR k). rewrite HSome in HR.
+      destruct (m1 !! k); [by eauto|done].
+  - intros [HR1 HR2] k.
+    destruct (m1 !! k) as [v1|] eqn:Heqn1.
+    { by apply HR1 in Heqn1 as [? [-> ?]]. }
+    destruct (m2 !! k) as [v2|] eqn:Heqn2.
+    { apply HR2 in Heqn2 as [? [? ?]]. by simplify_eq. }
+    done.
+Qed.
+
+Lemma map_included_delete `{Countable K} {V}
+      (R : relation V) (m1 m2 : gmap K V) k :
+  map_included R m1 m2 →
+  map_included R (delete k m1) (delete k m2).
+Proof.
+  rewrite !map_included_spec.
+  intros Hle k' v HSome.
+  apply lookup_delete_Some in HSome as [HK HSome].
+  apply Hle in HSome as (?&?&?).
+  exists x. by rewrite lookup_delete_ne.
+Qed.
+
+Lemma map_agree_R_dom `{Countable K} {V}
+      (R : relation V) (m1 m2 : gmap K V) :
+  map_agree_R R m1 m2 → dom m1 = dom m2.
+Proof.
+  rewrite map_agree_R_spec. intros [Hle1 Hle2]. apply set_eq.
+  intros k. split.
+  - intros [v1 HSome1]%elem_of_dom.
+    apply Hle1 in HSome1 as (?&?&?).
+    by apply elem_of_dom.
+  - intros [v2 HSome2]%elem_of_dom.
+    apply Hle2 in HSome2 as (?&?&?).
+    by apply elem_of_dom.
+Qed.
+
+Lemma map_agree_R_insert `{Countable K} {V}
+      (R : relation V) (m1 m2 : gmap K V) k v1 v2 :
+  R v1 v2 →
+  map_agree_R R m1 m2 →
+  map_agree_R R (<[k:=v1]>m1) (<[k:=v2]>m2).
+Proof.
+  rewrite !map_agree_R_spec.
+  intros HR [Hle1 Hle2].
+  split.
+  - intros k' v1' HSome1.
+    destruct (decide (k = k')) as [->|Hneq].
+    + rewrite lookup_insert in HSome1. simplify_eq.
+      exists v2. rewrite lookup_insert. done.
+    + rewrite lookup_insert_ne in HSome1; [done|].
+      apply Hle1 in HSome1 as (v2'&HSome2&HR2).
+      exists v2'. rewrite lookup_insert_ne; [|done]. done.
+  - intros k' v2' HSome2.
+    destruct (decide (k = k')) as [->|Hneq].
+    + rewrite lookup_insert in HSome2. simplify_eq.
+      exists v1. rewrite lookup_insert. done.
+    + rewrite lookup_insert_ne in HSome2; [done|].
+      apply Hle2 in HSome2 as (v1'&HSome1&HR1).
+      exists v1'. rewrite lookup_insert_ne; [|done]. done.
+Qed.
+
+Lemma map_agree_R_insert_inv `{Countable K} {V}
+      (R : relation V) (m1 m2 : gmap K V) k v1 v2 :
+  k ∉ dom m1 → k ∉ dom m2 →
+  map_agree_R R (<[k:=v1]>m1) (<[k:=v2]>m2) →
+  map_agree_R R m1 m2.
+Proof.
+  intros Hnin1 Hnin2.
+  rewrite !map_agree_R_spec.
+  intros [Hle1 Hle2].
+  split.
+  - intros k' v1' HSome1.
+    destruct (decide (k = k')) as [->|Hneq].
+    { apply not_elem_of_dom in Hnin1. set_solver. }
+    assert (<[k:=v1]>m1 !! k' = Some v1') as HSome1'.
+    { by rewrite lookup_insert_ne. }
+    apply Hle1 in HSome1' as (v2'&HSome2&HR).
+    rewrite lookup_insert_ne in HSome2; [done|].
+    by eauto.
+  - intros k' v2' HSome2.
+    destruct (decide (k = k')) as [->|Hneq].
+    { apply not_elem_of_dom in Hnin2. set_solver. }
+    assert (<[k:=v2]>m2 !! k' = Some v2') as HSome2'.
+    { by rewrite lookup_insert_ne. }
+    apply Hle2 in HSome2' as (v1'&HSome1&HR).
+    rewrite lookup_insert_ne in HSome1; [done|].
+    by eauto.
+Qed.
+
+Lemma map_agree_R_agree `{Countable K} {V}
+      (R : relation V) (m1 m2 : gmap K V) k v1 v2 :
+  m1 !! k = Some v1 → m2 !! k = Some v2 →
+  map_agree_R R m1 m2 →
+  R v1 v2.
+Proof.
+  rewrite map_agree_R_spec.
+  intros HSome1 HSome2 Hle.
+  apply Hle in HSome1 as (v2'&HSome2'&HR).
+  rewrite HSome2' in HSome2. by simplify_eq.
+Qed.
+
+Lemma map_included_R_agree `{Countable K} {V}
+      (R : relation V) (m1 m2 : gmap K V) k v1 v2 :
+  m1 !! k = Some v1 → m2 !! k = Some v2 →
+  map_included R m1 m2 →
+  R v1 v2.
+Proof.
+  rewrite map_included_spec.
+  intros HSome1 HSome2 Hle.
+  apply Hle in HSome1 as (v2'&HSome2'&HR).
+  rewrite HSome2' in HSome2. by simplify_eq.
+Qed.
+
+Lemma map_included_map_agree_R `{Countable K} {V}
+      (R : relation V) (m1 m2 : gmap K V) :
+  map_included R m1 m2 →
+  ∃ m21 m22,
+    m2 = m21 ∪ m22 ∧
+    m21 ##ₘ m22 ∧
+    map_agree_R R m1 m21.
+Proof.
+  revert m1.
+  induction m2 as [|k v2 m2 Hnin IHm2] using map_ind; intros m1 Hle.
+  { by exists ∅, ∅. }
+  destruct (decide (k ∈ dom m1)) as [Hin|Hnin']; last first.
+  { apply (map_included_delete _ _ _ k) in Hle.
+    rewrite delete_insert in Hle; [done|].
+    apply IHm2 in Hle as (m21&m22&->&Hdisj&HR).
+    exists m21, (<[k:=v2]>m22).
+    assert (dom m1 = dom m21) as Hdom.
+    { eapply map_agree_R_dom. apply not_elem_of_dom in Hnin'.
+      by rewrite delete_notin in HR. }
+    apply map_disjoint_dom in Hdisj.
+    rewrite insert_union_r; [by apply not_elem_of_dom; set_solver|].
+    split; [done|].
+    apply not_elem_of_dom in Hnin'.
+    rewrite delete_notin in HR; [done|].
+    split; [|done].
+    apply map_disjoint_dom.
+    apply not_elem_of_dom in Hnin'.
+    set_solver. }
+  apply elem_of_dom in Hin as [v1 HSome].
+  assert (R v1 v2).
+  { eapply map_included_R_agree; [| |done].
+    - done.
+    - by rewrite lookup_insert. }
+  apply (map_included_delete _ _ _ k) in Hle.
+  rewrite delete_insert in Hle; [done|].
+  apply IHm2 in Hle as (m21&m22&->&Hdisj&HR).
+  exists (<[k:=v2]>m21), m22.
+  assert (dom (delete k m1) = dom m21) as Hdom.
+  { eapply map_agree_R_dom. done. }
+  apply map_disjoint_dom in Hdisj.
+  rewrite insert_union_l.
+  split; [done|].
+  apply (map_agree_R_insert _ _ _ k v1 v2) in HR; [|done].
+  rewrite insert_delete in HR; [done|].
+  split; [|done].
+  apply map_disjoint_dom.
+  rewrite dom_insert_L.
+  apply not_elem_of_dom in Hnin.
+  set_solver.
+Qed.
+
+Lemma map_agree_R_map_included `{Countable K} {V}
+      (R : relation V) (m1 m2 : gmap K V) :
+  map_agree_R R m1 m2 → map_included R m1 m2.
+Proof.
+  rewrite map_included_spec map_agree_R_spec.
+  by intros [Hle _].
+Qed.
+
+Lemma map_agree_R_union_inv `{Countable K} {V}
+      (R : relation V) (m11 m12 m2 : gmap K V) :
+  m11 ##ₘ m12 →
+  map_agree_R R (m11 ∪ m12) m2 →
+  ∃ m21 m22, m2 = m21 ∪ m22 ∧ map_agree_R R m11 m21 ∧
+             map_agree_R R m12 m22.
+Proof.
+  intros Hdisj%map_disjoint_dom Hle.
+  pose proof Hle as Hdom%map_agree_R_dom.
+  rewrite comm in Hdom.
+  rewrite dom_union_L in Hdom.
+  apply dom_union_inv_L in Hdom as (m21&m22&->&Hdosj&Hdom1&Hdom2);
+    [|done].
+  exists m21, m22.
+  split; [done|].
+  split.
+  - apply map_agree_R_spec.
+    split.
+    + intros k v1 HSome1.
+      apply map_agree_R_spec in Hle as [Hle1 Hle2].
+      assert ((m11 ∪ m12) !! k = Some v1) as HSome1'.
+      { rewrite lookup_union_l; [|done].
+        apply not_elem_of_dom.
+        apply elem_of_dom_2 in HSome1. set_solver. }
+      apply Hle1 in HSome1' as (v2&HSome2'&HR).
+      assert (m21 !! k = Some v2) as HSome2.
+      { rewrite lookup_union_l in HSome2'; [|done].
+        apply not_elem_of_dom. apply elem_of_dom_2 in HSome1.
+        set_solver. }
+      eauto.
+    + intros k v2 HSome2.
+      apply map_agree_R_spec in Hle as [Hle1 Hle2].
+      assert ((m21 ∪ m22) !! k = Some v2) as HSome2'.
+      { rewrite lookup_union_l; [|done].
+        apply not_elem_of_dom.
+        apply elem_of_dom_2 in HSome2. set_solver. }
+      apply Hle2 in HSome2' as (v1&HSome1'&HR).
+      assert (m11 !! k = Some v1) as HSome1.
+      { rewrite lookup_union_l in HSome1'; [|done].
+        apply not_elem_of_dom. apply elem_of_dom_2 in HSome2.
+        set_solver. }
+      eauto.
+  - apply map_agree_R_spec.
+    split.
+    + intros k v1 HSome1.
+      apply map_agree_R_spec in Hle as [Hle1 Hle2].
+      assert ((m11 ∪ m12) !! k = Some v1) as HSome1'.
+      { rewrite lookup_union_r; [|done].
+        apply not_elem_of_dom.
+        apply elem_of_dom_2 in HSome1. set_solver. }
+      apply Hle1 in HSome1' as (v2&HSome2'&HR).
+      assert (m22 !! k = Some v2) as HSome2.
+      { rewrite lookup_union_r in HSome2'; [|done].
+        apply not_elem_of_dom. apply elem_of_dom_2 in HSome1.
+        set_solver. }
+      eauto.
+    + intros k v2 HSome2.
+      apply map_agree_R_spec in Hle as [Hle1 Hle2].
+      assert ((m21 ∪ m22) !! k = Some v2) as HSome2'.
+      { rewrite lookup_union_r; [|done].
+        apply not_elem_of_dom.
+        apply elem_of_dom_2 in HSome2. set_solver. }
+      apply Hle2 in HSome2' as (v1&HSome1'&HR).
+      assert (m12 !! k = Some v1) as HSome1.
+      { rewrite lookup_union_r in HSome1'; [|done].
+        apply not_elem_of_dom. apply elem_of_dom_2 in HSome2.
+        set_solver. }
+      eauto.
+Qed.
+
+(* OBS: Need restrictions on f *)
+Lemma map_agree_R_fmap_inv `{Countable K} {V}
+      (R : relation V) (m1 m2 : gmap K V) f :
+  (* OBS: Is this a general relation/function property? *)
+  (∀ v1 v2, R (f v1) v2 → ∃ v2', v2 = f v2') →
+  map_agree_R R (f <$> m1) m2 →
+  ∃ m2', m2 = f <$> m2'.
+Proof.
+  revert m1.
+  induction m2 as [|k v2 m2 Hnin IHm2] using map_ind; intros m1 Hf Hle.
+  { exists ∅. rewrite fmap_empty. done. }
+  pose proof Hle as Hle'.
+  apply map_agree_R_spec in Hle.
+  assert (<[k:=v2]> m2 !! k = Some v2) as HSome2
+                                            by by rewrite lookup_insert.
+  apply Hle in HSome2 as (v1&HSome1&HR).
+  apply lookup_fmap_Some in HSome1 as (v1'&<-&HSome1').
+  assert (∃ v2', v2 = f v2') as [v2' Heq].
+  { by eapply Hf. }
+  rewrite Heq in HR.
+  assert (map_agree_R R (f <$> (delete k m1)) m2) as Hle''.
+  { rewrite -(insert_id m1 k v1') in Hle'; [done|].
+    rewrite -insert_delete_insert in Hle'.
+    rewrite fmap_insert in Hle'.
+    eapply map_agree_R_insert_inv; [| |apply Hle'].
+    - set_solver.
+    - apply not_elem_of_dom. set_solver.
+  }
+  apply IHm2 in Hle'' as [m2' Heq']; [|done].
+  exists (<[k:=v2']>m2').
+  rewrite fmap_insert. rewrite Heq. f_equiv. done.
+Qed.
+
+(* OBS: Need restrictions on f *)
+Lemma map_agree_R_fmap `{Countable K} {V}
+      (R : relation V) (m1 m2 : gmap K V) f :
+  (∀ v1 v2, R (f v1) (f v2) → R v1 v2) →
+  map_agree_R R (f <$> m1) (f <$> m2) →
+  map_agree_R R m1 m2.
+Proof.
+  intros Hf.
+  rewrite !map_agree_R_spec.
+  intros [Hle1 Hle2].
+  split.
+  - intros k v1 HSome1.
+    assert ((f <$> m1) !! k = Some (f v1)) as HSome1'.
+    { rewrite lookup_fmap. destruct (m1 !! k); [by simplify_eq|done]. }
+    apply Hle1 in HSome1' as (v2'&HSome2'&HR).
+    apply lookup_fmap_Some in HSome2' as (v2&<-&HSome2).
+    apply Hf in HR.
+    by eauto.
+  - intros k v2 HSome2.
+    assert ((f <$> m2) !! k = Some (f v2)) as HSome2'.
+    { rewrite lookup_fmap. destruct (m2 !! k); [by simplify_eq|done]. }
+    apply Hle2 in HSome2' as (v1'&HSome1'&HR).
+    apply lookup_fmap_Some in HSome1' as (v1&<-&HSome1).
+    apply Hf in HR.
+    by eauto.
+Qed.
+
